chore: use `GetElem` everywhere
I don't like writing `fun _ _ ↦ True` everywhere, but I don't have any other way to make it interact well with `GetElem`...

Algorithm/Data/Classes/IndexedMinHeap.lean
@@ -9,20 +9,20 @@ import Algorithm.Data.Classes.ToList
 import Mathlib.Data.Prod.Lex
 
 class IndexedMinHeap (C : Type*) [Inhabited C] (ι : outParam Type*)
-    (α : outParam Type*) [Preorder α] [IsTotal α (· ≤ ·)] [OrderTop α] extends
-    AssocDArray C ι α fun _ ↦ ⊤ where
+    (α : outParam Type*) (V : outParam _) [Preorder α] [IsTotal α (· ≤ ·)] [OrderTop α] extends
+    AssocDArray C ι α V fun _ ↦ ⊤ where
   minIdx : C → ι
   getElem_minIdx_le c (i : ι) : c[minIdx c] ≤ c[i]
-  decreaseKey (c : C) (i : ι) : ∀ v < c[i], C := fun v _ ↦ set c i v
-  decreaseKey_eq_set (c : C) (i : ι) v (h : v < c[i]) : decreaseKey c i v h = set c i v := by
+  decreaseKey (c : C) (i : ι) : ∀ v < c[i], C := fun v _ ↦ c[i ↦ v]
+  decreaseKey_eq_set (c : C) (i : ι) v (h : v < c[i]) : decreaseKey c i v h = c[i ↦ v] := by
     intros; rfl
 export IndexedMinHeap (minIdx getElem_minIdx_le decreaseKey decreaseKey_eq_set)
 
 attribute [simp] decreaseKey_eq_set
 
 section IndexedMinHeap
-variable {C : Type*} [Inhabited C] {ι : Type*} {α : Type*} [LinearOrder α] [OrderTop α]
-  [IndexedMinHeap C ι α]
+variable {C : Type*} [Inhabited C] {ι : Type*} {α : Type*} {V} [LinearOrder α] [OrderTop α]
+  [IndexedMinHeap C ι α V]
 
 def decreaseKeyD (c : C) (i : ι) (v : α) : C :=
   if c[i] ≤ v then c else c[i ↦ v]
@@ -58,11 +58,11 @@ lemma decreaseKeysD_getElem [DecidableEq ι] {ια : Type*} [ToList ια (ι × 
 end IndexedMinHeap
 
 namespace Batteries.Vector
-variable {α : Type*} [LinearOrder α] {n : ℕ} [NeZero n] {d : Fin n → α}
+variable {α : Type*} [LinearOrder α] {n : ℕ} [NeZero n] {V} {d : Fin n → α}
 
 section ReadOnly
 
-variable [AssocDArray.ReadOnly (Vector α n) (Fin n) α d]
+variable [AssocDArray.ReadOnly (Vector α n) (Fin n) α V d]
 
 abbrev minAux (a : Vector α n) : Lex (α × Fin n) :=
   (⊤ : Finset (Fin n)).inf' ⟨0, Finset.mem_univ 0⟩ (fun i ↦ toLex (a[i], i))
@@ -90,7 +90,9 @@ lemma minIdx_le (a : Vector α n) (i : Fin n) :
 
 end ReadOnly
 
-instance [OrderTop α] : IndexedMinHeap (Vector.WithDefault α n fun _ ↦ ⊤) (Fin n) α where
+instance WithDefault.instIndexedMinHeap [OrderTop α] :
+    IndexedMinHeap (Vector.WithDefault α n fun _ ↦ ⊤) (Fin n) α (fun _ i ↦ (i : ℕ) < n) where
+  toAssocDArray := instAssocDArray
   minIdx := minIdx
   getElem_minIdx_le a i := a.minIdx_le i
 
@@ -143,8 +145,8 @@ instance [Preorder α] [IsTotal α (· ≤ ·)] :
 
 end AssocArrayWithHeap.WithIdx
 
-structure AssocArrayWithHeap (C C' : Type*) {ι α : Type*} [Preorder α] [IsTotal α (· ≤ ·)]
-    [Inhabited C] [AssocArray C ι (WithTop α) ⊤]
+structure AssocArrayWithHeap (C C' : Type*) {ι α : Type*} {V} [Preorder α] [IsTotal α (· ≤ ·)]
+    [Inhabited C] [AssocArray C ι (WithTop α) V ⊤]
     [MinHeap C' (AssocArrayWithHeap.WithIdx α ι)] where mk' ::
   assocArray : C
   minHeap : C'
@@ -153,14 +155,14 @@ structure AssocArrayWithHeap (C C' : Type*) {ι α : Type*} [Preorder α] [IsTot
     assocArray[(MinHeap.head minHeap h).idx] = (MinHeap.head minHeap h).val
 
 namespace AssocArrayWithHeap
-variable {C C' : Type*} {ι α : Type*} [Preorder α] [IsTotal α (· ≤ ·)]
-  [Inhabited C] [AssocArray C ι (WithTop α) ⊤]
+variable {C C' : Type*} {ι α : Type*} {V} [Preorder α] [IsTotal α (· ≤ ·)]
+  [Inhabited C] [AssocArray C ι (WithTop α) V ⊤]
   [MinHeap C' (AssocArrayWithHeap.WithIdx α ι)]
 
-instance : AssocArray.ReadOnly (AssocArrayWithHeap C C') ι (WithTop α) ⊤ where
-  get c := AssocArray.get c.assocArray
+instance : AssocArray.ReadOnly (AssocArrayWithHeap C C') ι (WithTop α) (fun _ _ ↦ True) ⊤ where
+  getElem c i _ := c.assocArray[i]
   toDFinsupp' c := toDFinsupp' c.assocArray
-  coe_toDFinsupp'_eq_get c := coe_toDFinsupp'_eq_get c.assocArray
+  coe_toDFinsupp'_eq_getElem c := coe_toDFinsupp'_eq_getElem c.assocArray
 
 @[simp]
 lemma assocArray_getElem (c : AssocArrayWithHeap C C') (i : ι) :
@@ -222,8 +224,9 @@ lemma default_minHeap :
     (default : AssocArrayWithHeap C C').minHeap = ∅ :=
   rfl
 
-instance [DecidableEq α] : AssocArray (AssocArrayWithHeap C C') ι (WithTop α) ⊤ where
-  set c i x :=
+instance [DecidableEq α] :
+    AssocArray (AssocArrayWithHeap C C') ι (WithTop α) (fun _ _ ↦ True) ⊤ where
+  setElem c i x :=
     mk
       c.assocArray[i ↦ x]
       (if hx : x = ⊤ then c.minHeap else insert ⟨x.untop hx, i⟩ c.minHeap)
@@ -231,7 +234,7 @@ instance [DecidableEq α] : AssocArray (AssocArrayWithHeap C C') ι (WithTop α)
         haveI : DecidableEq ι := by classical infer_instance
         split_ifs with hx <;>
           simp? [Function.update_apply] at hj ⊢ says
-            simp only [getElem_set, assocArray_getElem, ne_eq] at hj ⊢
+            simp only [all_valid, getElem_setElem, assocArray_getElem, ne_eq] at hj ⊢
         · subst hx
           rw [ite_eq_left_iff, Classical.not_imp] at hj
           simp only [hj.1, ↓reduceIte]
@@ -240,17 +243,17 @@ instance [DecidableEq α] : AssocArray (AssocArrayWithHeap C C') ι (WithTop α)
           split_ifs at hj ⊢ with hji
           · simp [hji]
           · exact .inr <| c.mem_minHeap j hj
-  get_set_eq _ _ _ := by simp [Get.get]
-  get_set_ne _ _ _ _ _ := by simp [Get.get, *]
-  get_default := by simp [Get.get]
+  getElem_setElem_self _ _ _ := by simp [getElem]
+  getElem_setElem_of_ne _ _ _ _ _ _ _ := by simp only [getElem]; simp [*]
+  getElem_default := by simp [getElem]
 
 @[simp]
-lemma set_assocArray [DecidableEq α] (c : AssocArrayWithHeap C C') (i x) :
+lemma set_assocArray [DecidableEq α] (c : AssocArrayWithHeap C C') (i : ι) (x) :
     c[i ↦ x].assocArray = c.assocArray[i ↦ x] := by
   unfold_projs; simp
 
 instance [Inhabited ι] [DecidableEq α] :
-    IndexedMinHeap (AssocArrayWithHeap C C') ι (WithTop α) where
+    IndexedMinHeap (AssocArrayWithHeap C C') ι (WithTop α) (fun _ _ ↦ True) where
   minIdx c := if h : isEmpty c.minHeap then default else (MinHeap.head c.minHeap h).idx
   getElem_minIdx_le c i := by
     dsimp; split_ifs with h
