Algorithm/Tactic/Attr/Register.lean
@@ -1,0 +1,9 @@
+/-
+Copyright (c) 2024 Yuyang Zhao. All rights reserved.
+Released under Apache 2.0 license as described in the file LICENSE.
+Authors: Yuyang Zhao
+-/
+import Lean.Meta.Tactic.Simp.RegisterCommand
+
+/-- The simpset `get_elem_simps` is used by the tactic `get_elem_tactic_trivial`. -/
+register_simp_attr get_elem_simps
